examples/steel/arraystructs/ListExampleOOM.fst
@@ -6,15 +6,15 @@ open Steel.C.Ref
 open Steel.Effect
 module A = Steel.Effect.Atomic
 
-open FStar.PCM.POD
+open Steel.C.Opt
 open ListNodeOOM
 
 (*
 let ok
-  (#value:Ghost.erased (pod int'))
-  (#next:Ghost.erased (pod (option (ref' node node))))
+  (#value:Ghost.erased (option int'))
+  (#next:Ghost.erased (option (option (ref' node node))))
   (p: ref 'a node_pcm)
-: SteelT (q:ref 'a (pod_pcm int'){q == ref_focus p _value})
+: SteelT (q:ref 'a (opt_pcm #int'){q == ref_focus p _value})
     (p `pts_to` mk_node value next)
     (fun q ->
        (p `pts_to` mk_node none next) `star`
@@ -23,10 +23,10 @@ let ok
 *)
 
 let oom
-  (#value:Ghost.erased (pod int'))
-  (#next:Ghost.erased (pod (option (ref' node node))))
+  (#value:Ghost.erased (option int'))
+  (#next:Ghost.erased (option (option (ref' node node))))
   (p: ref 'a node_pcm)
-: SteelT (q:ref 'a (pod_pcm (option (ref' node node))){q == ref_focus p _next})
+: SteelT (q:ref 'a (opt_pcm #(option (ref' node node))){q == ref_focus p _next})
     (p `pts_to` mk_node value next)
     (fun q ->
        (p `pts_to` mk_node value none) `star`
