examples/steel/arraystructs/ListNode.fsti
@@ -1,10 +1,10 @@
 module ListNode
 
-open FStar.PCM.POD
 open FStar.PCM
 open Steel.Effect
 open PointStruct
 open Steel.C.PCM
+open Steel.C.Opt
 open Steel.C.Ref
 open Steel.C.Connection
 module U = FStar.Universe
@@ -25,51 +25,51 @@ val node_pcm: pcm node
 /// (mk_node value next) represents (struct node){.value = value, .next = next}
 
 val mk_node
-  (i: Ghost.erased (pod int'))
-  (next: Ghost.erased (pod (option (ref' node node))))
+  (i: Ghost.erased (option int'))
+  (next: Ghost.erased (option (option (ref' node node))))
 : Ghost.erased node
 
 /// Lenses for fields
 
-val _value: node_pcm `connection` pod_pcm int'
-val _next: node_pcm `connection` pod_pcm (option (ref' node node))
+val _value: node_pcm `connection` opt_pcm #int'
+val _next: node_pcm `connection` opt_pcm #(option (ref' node node))
 
 /// Taking pointers to the fields of a node
 
 val addr_of_value
-  (#value:Ghost.erased (pod int'))
-  (#next:Ghost.erased (pod (option (ref' node node))))
+  (#value:Ghost.erased (option int'))
+  (#next:Ghost.erased (option (option (ref' node node))))
   (p: ref 'a node_pcm)
-: SteelT (q:ref 'a (pod_pcm int'){q == ref_focus p _value})
+: SteelT (q:ref 'a (opt_pcm #int'){q == ref_focus p _value})
     (p `pts_to` mk_node value next)
     (fun q ->
        (p `pts_to` mk_node none next) `star`
        (q `pts_to` value))
 
 val unaddr_of_value
-  (#value:Ghost.erased (pod int'))
-  (#next:Ghost.erased (pod (option (ref' node node))))
+  (#value:Ghost.erased (option int'))
+  (#next:Ghost.erased (option (option (ref' node node))))
   (p: ref 'a node_pcm)
-  (q: ref 'a (pod_pcm int'){q == ref_focus p _value})
+  (q: ref 'a (opt_pcm #int'){q == ref_focus p _value})
 : SteelT unit
     ((p `pts_to` mk_node none next) `star` (q `pts_to` value))
     (fun q -> p `pts_to` mk_node value next)
 
 val addr_of_next
-  (#value:Ghost.erased (pod int'))
-  (#next:Ghost.erased (pod (option (ref' node node))))
+  (#value:Ghost.erased (option int'))
+  (#next:Ghost.erased (option (option (ref' node node))))
   (p: ref 'a node_pcm)
-: SteelT (q:ref 'a (pod_pcm (option (ref' node node))){q == ref_focus p _next})
+: SteelT (q:ref 'a (opt_pcm #(option (ref' node node))){q == ref_focus p _next})
     (p `pts_to` mk_node value next)
     (fun q ->
        (p `pts_to` mk_node value none) `star`
        (q `pts_to` next))
 
 val unaddr_of_next
-  (#value:Ghost.erased (pod int'))
-  (#next:Ghost.erased (pod (option (ref' node node))))
+  (#value:Ghost.erased (option int'))
+  (#next:Ghost.erased (option (option (ref' node node))))
   (p: ref 'a node_pcm)
-  (q: ref 'a (pod_pcm (option (ref' node node))){q == ref_focus p _next})
+  (q: ref 'a (opt_pcm #(option (ref' node node))){q == ref_focus p _next})
 : SteelT unit
     ((p `pts_to` mk_node value none) `star` (q `pts_to` next))
     (fun q -> p `pts_to` mk_node value next)
